% =============================================================================
\chapter{Functional calculus}
% =============================================================================

Phase-space treatment of multimode problems can be simplified by working with multimode field operators instead of single-mode operators.
It was initially introduced by Graham~\cite{Graham1970,Graham1970a}.
Examples of usage can be found in ~\cite{Steel1998,Norrie2006a}.
Detailed description of functional calculus is given in~\cite{Dalton2011} \todo{anywhere else?}.
Here we only provide some important results which are going to be used later on in this chapter.
\todo{Move to bibliography review and extend.}

First we must introduce some operations on functions, which will replace common differentials and integrals used in single and multi-mode cases and help encapsulate basis and mode populations inside wave functions and field operators.
In order to do that, we define an orthonormal basis $\fullbasis$ consisting of functions $\phi_{\nvec}(\xvec)$, where $\xvec \in \mathbb{R}^D$ is a coordinate vector, and $\nvec \in \fullbasis$ is a mode identifier.
Orthonormality and completeness conditions for basis functions are, respectively,
\begin{eqns}
	\int\limits_A \phi_{\nvec}^*(\xvec) \phi_{\mvec}(\xvec) d\xvec & = \delta_{\nvec\mvec}, \\
	\sum_{\nvec} \phi_{\nvec}^*(\xvec) \phi_{\nvec}(\xvec^\prime) & = \delta(\xvec^\prime - \xvec),
\end{eqns}
where the exact nature of integration area $A$ depends on the nature of the basis set
(for example, $A$ is the whole space for harmonic oscillator modes, and a box for plane waves).
Hereinafter we assume that the integration $\int d\xvec$ is always performed over $A$.

In order to avoid clutter, functions of coordinates will be dubbed as $f \equiv f(\xvec)$ and $f^\prime \equiv f(\xvec^\prime)$ except where it is necessary for clarity.

\begin{definition}
	$\mathbb{F}_{\restbasis}$ is a space of all functions of coordinates, which consists only of modes from $\restbasis$: $\mathbb{F}_{\restbasis} \equiv (\mathbb{R}^D \rightarrow \mathbb{C})_{\restbasis}$ (restricted functions).
	We denote $\mathbb{F}_{\fullbasis} \equiv \mathbb{F}$.
\end{definition}

Now we can define the composition transformation.

\begin{definition}
	Composition transformation creates a function from a vector of mode populations:
	\begin{eqn*}
		& \mathcal{C}_{\restbasis} :: \mathbb{C}^{|\restbasis|} \rightarrow \mathbb{F}_{\restbasis} \\
		& \mathcal{C}_{\restbasis}(\balpha) = \sum_{\nvec \in \restbasis} \phi_{\nvec} \alpha_{\nvec}.
	\end{eqn*}
	Decomposition transformation, correspondingly, creates a vector of populations out of a function:
	\begin{eqn*}
		& \mathcal{C}_{\restbasis}^{-1} :: \mathbb{F} \rightarrow \mathbb{C}^{|\restbasis|} \\
		& (\mathcal{C}_{\restbasis}^{-1}[f])_{\nvec}
		= \int d\xvec \phi_{\nvec}^* f,\,{\nvec} \in \restbasis.
	\end{eqn*}
	Note that for any $f \in \mathbb{F}_{\restbasis}$, $\mathcal{C}_{\restbasis}(\mathcal{C}_{\restbasis}^{-1}[f]) \equiv f$.
\end{definition}

The result of any non-linear transformation of a function $f \in \mathbb{F}_{\restbasis}$ is not guaranteed to belong to $\mathbb{F}_{\restbasis}$ and requires explicit projection to be used with other restricted functions.
This applies to the delta function of coordinates.
To avoid confusion with the common delta function, we introduce the restricted delta function.

\begin{definition}
\label{def:func-calculus:restricted-delta}
	The restricted delta function $\delta_{\restbasis} \in \mathbb{F}_{\restbasis}$ is defined as
	\begin{eqn*}
		\delta_{\restbasis}(\xvec^\prime, \xvec)
		= \sum_{\nvec \in \restbasis} \phi_{\nvec}^{\prime*} \phi_{\nvec}.
	\end{eqn*}
	Note that $\delta_{\restbasis}^*(\xvec^\prime, \xvec) = \delta_{\restbasis}(\xvec, \xvec^\prime)$.
\end{definition}

Any function can be projected to $\restbasis$ using the projection transformation.

\begin{definition}
\label{def:func-calculus:projector}
	Projection transformation
	\begin{eqn*}
		& \mathcal{P}_{\restbasis} :: \mathbb{F} \rightarrow \mathbb{F}_{\restbasis} \\
		& \mathcal{P}_{\restbasis}[f](\xvec)
		= (\mathcal{C}_{\restbasis}(\mathcal{C}_{\restbasis}^{-1}[f])) (\xvec)
		= \sum_{\nvec \in \restbasis} \phi_{\nvec} \int
			d\xvec^\prime\, \phi_{\nvec}^{\prime*} f^\prime
		= \int d\xvec^\prime \delta_{\restbasis}(\xvec^\prime, \xvec) f^\prime,
	\end{eqn*}
	Obviously, $\mathcal{P}_{\fullbasis} \equiv \mathds{1}$.
\end{definition}

The conjugate of $\mathcal{P}_{\restbasis}$ is thus defined as
\begin{eqn}
	(\mathcal{P}_{\restbasis}[f](\xvec))^*
	= \int d\xvec^\prime \delta_{\restbasis}^*(\xvec^\prime, \xvec) f^{\prime*}
	= \mathcal{P}_{\restbasis}^* [f^*](\xvec).
\end{eqn}


% =============================================================================
\section{Functional differentiation}
% =============================================================================

Let $\mathcal{F}[f] :: \mathbb{F}_{\restbasis} \rightarrow \mathbb{F}$ be some transformation (note that the result is not guaranteed to belong to the restricted basis).
Because of the bijection between $\mathbb{F}_{\restbasis}$ and $\mathbb{C}^{|\restbasis|}$, $\mathcal{F}$ can be alternatively treated as a function of a vector of complex numbers:
\begin{eqn}
	& \mathcal{F} :: \mathbb{C}^{|\restbasis|} \rightarrow \mathbb{C}^\infty \\
	& \mathcal{F}(\balpha) \equiv \mathcal{C}_{\restbasis}^{-1}[\mathcal{F}[\mathcal{C}_{\restbasis}(\balpha)]].
\end{eqn}
Using this correspondence, we can define the functional differentiation.

\begin{definition}
\label{def:func-calculus:func-diff}
	Functional derivative is defined as
	\begin{eqn*}
		& \frac{\delta}{\delta f^\prime} ::
		\left(
			\mathbb{F}_{\restbasis} \rightarrow \mathbb{F}
		\right)
		\rightarrow
		\left(
			\mathbb{R}^D \rightarrow \mathbb{F}_{\restbasis} \rightarrow \mathbb{F}
		\right) \\
		& \frac{\delta \mathcal{F}[f]}{\delta f^\prime}
		= \sum_{\nvec \in \restbasis} \phi_{\nvec}^{\prime*}
			\frac{\partial \mathcal{F}(\balpha)}{\partial \alpha_{\nvec}}.
	\end{eqn*}
\end{definition}

Note that the transformation being returned differs from the one which was taken:
the result of new transformation is a function depending on two variables from $\mathbb{R}^D$, not one.
The second variable comes from the function we are differentiating by.

Functional derivative definition behaves in many ways similar to common derivative.
\begin{lemma}
	Functional differentiation from~\defref{func-calculus:func-diff} obeys sum, product, quotient, and chain differentiation rules.
\end{lemma}
\begin{proof}
\todo{Sum, product and quotient are more or less obvious; but should we prove chain differentiation?}
\end{proof}

\begin{lemma}
	If $g(t)$ is a function that can be expanded into power series, and functional $\mathcal{F}[f] \equiv g(f)$, $\mathcal{F} \in \mathbb{F}_{\restbasis} \rightarrow \mathbb{F}$, then
	\begin{eqn*}
		\frac{\delta \mathcal{F}[f]}{\delta f(\xvec^\prime)} (\xvec)
		= \delta_{\restbasis}(\xvec^\prime - \xvec)
			\left. \frac{\partial g(t)}{\partial t} \right|_{t = f(\xvec)}
	\end{eqn*}
\end{lemma}
\begin{proof}
We will consider $g(t) = t^k$ case first, which will straightforwardly lead to the statement of the lemma.
For $k = 1$, obviously,
\begin{eqn}
	\frac{\delta f}{\delta f(\xvec^\prime)} (\xvec)
	= \delta_{\restbasis}(\xvec^\prime, \xvec)
\end{eqn}
Then for other values of $k$:
\begin{eqn}
	\frac{\delta \mathcal{F}[f]}{\delta f(\xvec^\prime)} (\xvec)
	& = \frac{\delta f^k}{\delta f(\xvec^\prime)} (\xvec)
	= \sum_{\nvec \in \restbasis} \phi_{\nvec}^{\prime*}
		\frac{\partial f^k}{\partial \alpha_{\nvec}} \\
	& = \sum_{\nvec \in \restbasis} \phi_{\nvec}^{\prime*}
		\frac{\partial f^k}{\partial f}
		\frac{\partial f}{\partial \alpha_{\nvec}}
	= k f^{k-1}
		\sum_{\nvec \in \restbasis} \phi_{\nvec}^{\prime*}
		\frac{\partial f}{\partial \alpha_{\nvec}} \\
	& = k \delta_{\restbasis}(\xvec^\prime, \xvec) f^{k-1}(\xvec)
	= \delta_{\restbasis}(\xvec^\prime, \xvec)
		\left. \frac{\partial t^k}{\partial t} \right|_{t = f(\xvec)}.
	\qedhere
\end{eqn}
\end{proof}

\begin{lemma}
	If $g(z, z^*)$ can be expanded into series of $z^n (z^*)^m$, and functional $\mathcal{F}[f, f^*] \equiv g(f, f^*)$, $\mathcal{F} \in \mathbb{F}_{\restbasis} \rightarrow \mathbb{F}$, then $\delta \mathcal{F} / \delta f^\prime$ and $\delta \mathcal{F} / \delta f^{\prime*}$ can be treated as a partial differentiation of the functional of two independent variables $f$ and $f^*$.
	In other words:
	\begin{eqn*}
		\frac{\delta \mathcal{F}}{\delta f^\prime}
		= \delta_P(\xvec^\prime, \xvec) \left.
			\frac{\partial g(z, z^*)}{\partial z}
		\right|_{z=f(x)},
		\quad
		\frac{\delta \mathcal{F}}{\delta f^{\prime*}}
		= \delta_P^*(\xvec^\prime, \xvec) \left.
			\frac{\partial g(z, z^*)}{\partial z^*}
		\right|_{z=f(x)}
	\end{eqn*}
\end{lemma}
\begin{proof}
Proof is similar to \lmmref{c-numbers:independent-vars}.
\end{proof}


% =============================================================================
\section{Functional integration}
% =============================================================================

Functional integration is defined as

\begin{definition}
	\begin{eqn*}
		& \int \delta^2 f :: (\mathbb{F}_{\restbasis} \rightarrow \mathbb{F}) \rightarrow \mathbb{C} \\
		& \int \delta^2 f \mathcal{F}[f]
		= \int d^2\balpha \mathcal{F}(\balpha)
		= \left(
			\prod_{\nvec \in \restbasis} \int d^2\alpha_{\nvec}
		\right) \mathcal{F}(\balpha),
	\end{eqn*}
	where the product of integrals stands for their successive application.
    If the basis contains an infinite number of modes, the integral is treated as a limit $|\restbasis| \rightarrow \infty$.
	\todo{\cite{Dalton2011} has detailed explanation, do we need it here?}
\end{definition}

Functional integration has the Fourier-like property analogous to \lmmref{c-numbers:fourier-of-moments}, but its statement requires the definition of the delta functional:

\begin{definition}
\label{def:func-calculus:delta-functional}
	For a function $\Lambda \in \mathbb{F}_{\restbasis}$ the delta functional is
	\begin{eqn*}
		\Delta_{\restbasis}[\Lambda]
		\equiv \prod_{\nvec \in \restbasis} \delta(\Real \lambda_{\nvec}) \delta(\Imag \lambda_{\nvec}),
	\end{eqn*}
	where $\blambda = \mathcal{C}_{\restbasis}^{-1}[\Lambda]$.
\end{definition}

The delta functional has the same property as the common delta function:
\begin{eqn}
	\int \delta^2 \Lambda \mathcal{F}[\Lambda] \Delta_{\restbasis}[\Lambda]
	& = \left(
			\prod_{\nvec \in \restbasis} \int d^2\lambda_{\nvec}
		\right)
		\mathcal{F}(\blambda)
		\prod_{\nvec \in \restbasis} \delta(\Real \lambda_{\nvec}) \delta(\Imag \lambda_{\nvec}) \\
	& = \left. \mathcal{F}(\blambda) \right|_{\forall \nvec \in \restbasis\, \lambda_{\nvec} = 0} \\
	& = \left. \mathcal{F}[\Lambda] \right|_{\Lambda \equiv 0}
\end{eqn}

\begin{lemma}[Functional extension of \lmmref{c-numbers:fourier-of-moments}]
\label{lmm:func-calculus:fourier-of-moments}
	For $\Psi \in \mathbb{F}_{\restbasis}$ and $\Lambda \in \mathbb{F}_{\restbasis}$, and for any non-negative integers $r$ and $s$:
	\begin{eqn*}
		\int \delta^2\Psi\, \Psi^r (\Psi^*)^s \exp
			\int d\xvec \left( -\Lambda \Psi^* + \Lambda^* \Psi \right)
		= \pi^{2|\restbasis|}
			\left( -\frac{\delta}{\delta \Lambda^*} \right)^r
			\left( \frac{\delta}{\delta \Lambda} \right)^s
			\Delta_{\restbasis}[\Lambda]
	\end{eqn*}
\end{lemma}
\begin{proof}
\begin{eqn}
	& \int \delta^2\Psi\, \Psi^r (\Psi^*)^s \exp
		\int d\xvec \left( -\Lambda \Psi^* + \Lambda^* \Psi \right) \\
	& = \left(
			\prod_{\nvec \in \restbasis} \int d^2\alpha_{\nvec}
		\right)
		\left( \sum_{\nvec \in \restbasis} \phi_{\nvec} \alpha_{\nvec} \right)^r
		\left( \sum_{\nvec \in \restbasis} \phi^*_{\nvec} \alpha_{\nvec}^* \right)^s
		\prod_{\nvec \in \restbasis} \exp(-\lambda_{\nvec} \alpha_{\nvec}^* + \lambda_{\nvec}^* \alpha_{\nvec}).
\end{eqn}
Expanding powers of $\Psi$ and $\Psi^*$ using multinomial theorem:
\begin{eqn2}
	& ={} && \left(
			\prod_{\nvec \in \restbasis} \int d^2\alpha_{\nvec}
		\right)
		\left(
			\sum_{\sum u_{\mvec} = r} \binom{r}{ \left\{ u_{\mvec} \right\} }
			\prod_{\nvec \in \restbasis} \phi_{\nvec}^{u_{\nvec}} \alpha_{\nvec}^{u_{\nvec}}
		\right) \\
	& && \left(
			\sum_{\sum v_{\mvec} = s} \binom{s}{ \left\{ v_{\mvec} \right\} }
			\prod_{\nvec \in \restbasis} (\phi_{\nvec}^*)^{v_{\nvec}} (\alpha_{\nvec}^*)^{v_{\nvec}}
		\right)
		\prod_{\nvec \in \restbasis} \exp(-\lambda_{\nvec} \alpha_{\nvec}^* + \lambda_{\nvec}^* \alpha_{\nvec}),
\end{eqn2}
where $\binom{r}{ \left\{ u_{\mvec} \right\} } \equiv r! / (\prod u_{\mvec}!)$ are multinomial coefficients.
Splitting variables:
\begin{eqn2}
	& ={} && \sum_{ \sum u_{\mvec} = r,\, \sum v_{\mvec} = s }
		\binom{r}{ \left\{ u_{\mvec} \right\} }
		\binom{s}{ \left\{ v_{\mvec} \right\} } \\
	& && \prod_{\nvec \in \restbasis}
			\phi_{\nvec}^{u_{\nvec}} (\phi_{\nvec}^*)^{v_{\nvec}}
			\int d^2\alpha_{\nvec}
				\alpha_{\nvec}^{u_{\nvec}}
				(\alpha_{\nvec}^*)^{v_{\nvec}}
				\exp(-\lambda_{\nvec} \alpha_{\nvec}^* + \lambda_{\nvec}^* \alpha_{\nvec}).
\end{eqn2}
Applying \lmmref{c-numbers:fourier-of-moments}, collapsing sums, and recognizing \defref{func-calculus:func-diff} and \defref{func-calculus:delta-functional}:
\begin{eqn2}
	& ={} && \sum_{\sum u_{\mvec} = r,\, \sum v_{\mvec} = s}
		\binom{r}{ \left\{ u_{\mvec} \right\} }
		\binom{s}{ \left\{ v_{\mvec} \right\} }
		\pi^{2|\restbasis|} \\
	& && \prod_{\nvec \in \restbasis}
			\phi_{\nvec}^{u_{\nvec}} (\phi_{\nvec}^*)^{v_{\nvec}}
			\left( -\frac{\partial}{\partial \lambda_{\nvec}^*} \right)^{u_{\nvec}}
			\left( \frac{\partial}{\partial \lambda_{\nvec}} \right)^{v_{\nvec}}
			\delta(\Real \lambda_{\nvec}) \delta(\Imag \lambda_{\nvec}) \\
	& ={} && \pi^{2|\restbasis|}
		\left( -\sum_{\nvec \in \restbasis} \phi_{\nvec} \frac{\partial}{\partial \lambda_{\nvec}^*} \right)^r
		\left( \sum_{\nvec \in \restbasis} \phi_{\nvec}^* \frac{\partial}{\partial \lambda_{\nvec}} \right)^s
		\prod_{\nvec \in \restbasis} \delta(\Real \lambda_{\nvec}) \delta(\Imag \lambda_{\nvec}) \\
	& ={} && \pi^{2|\restbasis|}
		\left( -\frac{\delta}{\delta \Lambda^*} \right)^r
		\left( \frac{\delta}{\delta \Lambda} \right)^s
		\Delta_{\restbasis}[\Lambda]
	\qedhere
\end{eqn2}
\end{proof}

In order to perform transformations of master equations in the future, we will need a lemma, which justifies certain operation with Laplacian (which is a part of kinetic term in Hamiltonian).

\begin{lemma}
\label{lmm:func-calculus:move-laplacian}
	If $\forall \nvec \in \restbasis\, \xvec \in \partial A$ $\phi_n(\xvec) = 0$, then for any $\mathcal{F} \in \mathbb{F}_{\restbasis} \rightarrow \mathbb{F}$
	\begin{eqn*}
		\int\limits_A d\xvec \left(
			\nabla^2 \frac{\delta}{\delta \Psi}
		\right) \Psi \mathcal{F}[\Psi, \Psi^*]
		= \int\limits_A d\xvec \frac{\delta}{\delta \Psi}
		( \nabla^2 \Psi ) \mathcal{F}[\Psi, \Psi^*]
	\end{eqn*}
\end{lemma}
\begin{proof}
Integration limits play an important role in this proof, so we will write them explicitly.
\begin{eqn}
	\int\limits_A d\xvec \left(
		\nabla^2 \frac{\delta}{\delta \Psi}
	\right) \Psi
	= \sum_{\nvec \in \restbasis, \mvec \in \restbasis} \left(
			\int\limits_A d\xvec ( \nabla^2 \phi_{\nvec}^* ) \phi_{\mvec}
		\right)
		\frac{\partial}{\partial \alpha_{\nvec}} \alpha_{\mvec} \mathcal{F}(\bm{\alpha})
	= (*)
\end{eqn}
Using Green's first identity and the fact that eigenfunctions are equal to zero at the boundary of $A$:
\begin{eqn}
	\int\limits_A d\xvec ( \nabla^2 \phi_{\nvec}^* ) \phi_{\mvec}
	& = \oint\limits_{\partial A} \phi_{\mvec} (\nabla \phi_{\nvec}^* \cdot \bm{v}) dS
	- \int\limits_A d\xvec ( \nabla \phi_{\nvec}^* ) ( \nabla \phi_{\mvec} ) \\
	& = 0 - \int\limits_A d\xvec ( \nabla \phi_{\nvec}^* ) ( \nabla \phi_{\mvec} ) \\
	& = \oint\limits_{\partial A} \phi_{\nvec}^* (\nabla \phi_{\mvec} \cdot \bm{v}) dS
	- \int\limits_A d\xvec ( \nabla \phi_{\nvec}^* ) ( \nabla \phi_{\mvec} ) \\
	& = \int\limits_A d\xvec \phi_{\nvec}^* ( \nabla^2 \phi_{\mvec} ),
\end{eqn}
where $\bm{v}$ is the outward pointing unit normal of surface element $dS$.
Thus
\[
	(*)
	= \sum_{\nvec \in \restbasis, \mvec \in \restbasis} \left(
			\int\limits_A d\xvec \phi_{\nvec}^* ( \nabla^2 \phi_{\mvec} )
		\right)
		\frac{\partial}{\partial \alpha_{\nvec}} \alpha_{\mvec} \mathcal{F}(\bm{\alpha})
	= \int\limits_A d\xvec \frac{\delta}{\delta \Psi}
		( \nabla^2 \Psi ) \mathcal{F}[\Psi, \Psi^*].
	\qedhere
\]
\end{proof}

Note that this lemma imposes additional requirement for basis functions, but in practical applications it is always satisfied.
For example, in plane wave basis eigenfunctions are equal to zero at the border of the bounding box, and in harmonic oscillator basis they are equal to zero on the infinity (which can be considered the boundary of their integration area).
Hereinafter we will assume that this condition is true for any basis we work with.
