% =============================================================================
\section{Field operator calculus}
% =============================================================================

Description of complex bosonic systems with thousands of particles and strong nonlinear interactions often requires one to consider more than one mode per component.
Although it is quite possible to use single-mode creation and annihilation operators exclusively,
it is usually advantageous to employ a higher-level field operator representation.
Field operators can simplify both the analysis of a master equation, and its transformation to a Fokker-Planck equation (\abbrev{fpe}) using phase-space methods, which is the main topic of this thesis.

In this section we are going to outline the functional operator calculus, which is used extensively in this thesis.
This calculus is quite similar to the calculus of functional operators, described in \appref{func-calculus}).
The similartiy and interconnection of field operators and functional operators will become even more evident during the description of the functional Wigner transformation in \charef{wigner}.

Multimode fields are described by field operators $\Psiop_j^{\dagger}(\xvec)$ and $\Psiop_j(\xvec)$, where $\Psiop_j^{\dagger}$ creates a bosonic atom of spin $j$, $j = 1 \ldots C$ at location $\xvec$, and $\Psiop_j$ destroys one.
We will use the same scheme as with functions of coordinates in \appref{func-calculus}, abbreviating $\Psiop_j \equiv \Psiop_j(\xvec)$ and $\Psiop_j^\prime \equiv \Psiop_j(\xvec^\prime)$.

The commutators are
\begin{eqn}
\label{eqn:wigner:op-calculus:commutators}
    [ \Psiop_j, \Psiop_k^{\prime\dagger} ]
    = \delta_{jk} \delta(\xvec^\prime-\xvec).
\end{eqn}
Field operators have type $\Psiop_j \in (\mathbb{R}^D \rightarrow \mathbb{H}_j) = \mathbb{FH}_j$. \todo{As far as I understand $\mathbb{H}_1 \times \ldots \times \mathbb{H}_C \equiv \mathbb{H}$, where $\rho \in \mathbb{H}$.}
Field operators can be decomposed using a single-particle basis \todo{explanation needed?}:
\begin{eqn}
    \Psiop_j = \sum_{\nvec \in \fullbasis_j} \phi_{j,\nvec} \hat{a}_{j,\nvec}.
\end{eqn}
Note that each component can have its own basis.
Single mode operators $\hat{a}_{j,\nvec}$ obey commutation relations~\eqnref{wigner:mm-aux:commutators},
the pair $j,\nvec$ serving as a mode identifier.

We want to restrict ourselves only to a subset of modes from full basis for each component: $\restbasis_j \subset \fullbasis_j$ \todo{Or $\subseteq$ if we allow infinite $\restbasis$? This will lead to some mathematical difficulties}.
New restricted field operators are
\begin{eqn}
    \Psiop_j = \sum_{\nvec \in \restbasis_j} \phi_{j,\nvec} \hat{a}_{j,\nvec}.
\end{eqn}
They map coordinates to a restricted Hilbert subspaces: $\Psiop_j \in (\mathbb{R} \rightarrow \mathbb{H}_{\restbasis_j}) = \mathbb{FH}_{\restbasis_j}$.
Because of the restricted nature of these operators, commutation relations~\eqnref{wigner:op-calculus:commutators} no longer apply.
The following ones should be used instead:
\begin{eqn}
\label{eqn:wigner:op-calculus:restricted-commutators}
    \left[ \Psiop_j, \Psiop_k^\prime \right]
    & = \left[ \Psiop_j^\dagger, \Psiop_k^{\prime\dagger} \right] = 0, \\
    \left[ \Psiop_j, \Psiop_k^{\prime\dagger} \right]
    & = \delta_{jk} \delta_{\restbasis_j}(\xvec^\prime, \xvec).
\end{eqn}

Let us now find the expression for high-order commutators of restricted field operators, analogous to \lmmref{wigner:mm-aux:high-order-commutators} for single-mode operators.
It can be done using the similar recursive procedure.

\begin{lemma}
    For $\Psiop \in \mathbb{H}_{\restbasis}$
    \begin{eqn*}
        \left[ \Psiop, ( \Psiop^{\prime\dagger} )^l \right]
        & = l \delta_{\restbasis} (\xvec^\prime, \xvec) ( \Psiop^{\prime\dagger} )^{l-1}, \\
        \left[ \Psiop^\dagger, ( \Psiop^\prime )^l \right]
        & = - l \delta_{\restbasis}^* (\xvec^\prime, \xvec) ( \Psiop^\prime )^{l-1}.
    \end{eqn*}
\end{lemma}
\begin{proof}
Given that we know the expression for $\left[ \Psiop, ( \Psiop^{\prime\dagger} )^{l-1} \right]$,
the commutator of higher order can be expanded as
\begin{eqn}
    \left[ \Psiop, ( \Psiop^{\prime\dagger} )^l \right]
    & = \Psiop ( \Psiop^{\prime\dagger} )^l - ( \Psiop^{\prime\dagger} )^l \Psiop \\
    & = (
        \delta_{\restbasis} (\xvec^\prime, \xvec) + \Psiop^{\prime\dagger} \Psiop
    ) ( \Psiop^{\prime\dagger} )^{l-1}
    - ( \Psiop^{\prime\dagger} )^l \Psiop \\
    & = \delta_{\restbasis} (\xvec^\prime, \xvec) ( \Psiop^{\prime\dagger} )^{l-1}
    + \Psiop^{\prime\dagger} (
        \Psiop ( \Psiop^{\prime\dagger} )^{l-1}
        - ( \Psiop^{\prime\dagger} )^{l-1} \Psiop
    ) \\
    & = \delta_{\restbasis} (\xvec^\prime, \xvec) ( \Psiop^{\prime\dagger} )^{l-1}
    + \Psiop^{\prime\dagger} [
        \Psiop, ( \Psiop^{\prime\dagger} )^{l-1}
    ].
\end{eqn}
Now we can get the commutator of any order starting from the known relation~\eqnref{wigner:op-calculus:restricted-commutators}.
\end{proof}

A further generalisation of these relations is
\begin{lemma}
\label{lmm:wigner:op-calculus:functional-commutators}
    For $\Psiop \in \mathbb{H}_{\restbasis}$
    \begin{eqn*}
        \left[ \Psiop, f( \Psiop^\prime, \Psiop^{\prime\dagger} ) \right]
        & = \delta_{\restbasis} (\xvec^\prime, \xvec) \frac{\partial f}{\partial \Psiop^{\prime\dagger}}, \\
        \left[ \Psiop^\dagger, f( \Psiop^\prime, \Psiop^{\prime\dagger} ) \right]
        & = -\delta_{\restbasis}^* (\xvec^\prime, \xvec) \frac{\partial f}{\partial \Psiop^\prime},
    \end{eqn*}
    where $f(x, y)$ is a function that can be expanded in the power series of $x$ and $y$.
\end{lemma}
\begin{proof}
Let us prove the first relation; the procedure for the second one is the same.
Without loss of generality, we can assume that $f(\Psiop^\prime, \Psiop^{\prime\dagger})$ can be expanded in power series of normally ordered operators (otherwise we can just use commutation relations).
Thus
\begin{eqn}
    \left[ \Psiop, f( \Psiop^\prime, \Psiop^{\prime\dagger} ) \right]
    & = \sum_{r,s} f_{rs} [ \Psiop, (\Psiop^{\prime\dagger})^r (\Psiop^\prime)^s ] \\
    & = \sum_{r,s} f_{rs} [ \Psiop, (\Psiop^{\prime\dagger})^r ] (\Psiop^\prime)^s \\
    & = \sum_{r,s} f_{rs} r \delta_P(\xvec^\prime, \xvec)
        (\Psiop^{\prime\dagger})^{r-1} (\Psiop^\prime)^s \\
    & = \delta_P (\xvec^\prime, \xvec) \frac{\partial f}{\partial \Psiop^{\prime\dagger}}.
    \qedhere
\end{eqn}
\end{proof}
